lambda/examples/ex03_list/ex14_omega.v
@@ -1,0 +1,17 @@
+Require Import list_examples.
+
+Definition omega_cfg env s m k :=
+     {|
+     code := Exp ((Var 0) (Var 0)) (Env (Closure ((Var 0) (Var 0)) (Env env) :: env));
+     heap := s;
+     mark := m;
+     ctx := k |}.
+
+Inductive omega_spec : Spec cfg :=
+  omega_claim : forall F env s m k,
+    omega_spec (omega_cfg env s m k) (evals F m k (fun _ : val => constraint False)).
+
+Lemma omega_proof : sound lam_step omega_spec.
+Proof.
+  list_solver. contradiction. Grab Existential Variables. assumption.
+Qed.
